\section{Forward and Futures}


\subsection*{Forward Interest rates}
The forward interest rate between time $t-1$ and $t$ satisfies:\\
$ (1+r_t)^t = (1+r_{t-1})^{t-1}(1+f_t) $ \\
$ f_t = \frac{B_{t-1}}{B_t} -1 =\frac{(1+r_t)^t}{(1+r_{t-1})^{t-1}} -1 $


\subsection*{Forward price}
$F_T=e^{(r-y)T} S_0$


\subsection*{Swaps}
The swap rate is a weighted average of forward rates: \\
$r_s = \frac{\sum_{t=1}^{T}B_t f_t}{\sum_{u=1}^{T}B_u} = \sum_{t=1}^{T} w_t  f_t$ , 
with the weights $w_t \ \frac{B_t}{\sum_{u=1}^{T} B_u}$ \\